compiler/backend/proofs/data_to_word_assignProofScript.sml
@@ -8341,6 +8341,10 @@ val assign_FP_cmp = SIMP_CONV (srw_ss()) [assign_def]
   ``((assign (c:data_to_word$config) (secn:num) (l:num) (dest:num) (FP_cmp fpc)
        (args:num list) (names:num_set option)):'a wordLang$prog # num)``;
 
+val assign_FP_top = SIMP_CONV (srw_ss()) [assign_def]
+  ``((assign (c:data_to_word$config) (secn:num) (l:num) (dest:num) (FP_top fpt)
+       (args:num list) (names:num_set option)):'a wordLang$prog # num)``;
+
 val assign_FP_bop = SIMP_CONV (srw_ss()) [assign_def]
   ``((assign (c:data_to_word$config) (secn:num) (l:num) (dest:num) (FP_bop fpb)
        (args:num list) (names:num_set option)):'a wordLang$prog # num)``;
@@ -8483,6 +8487,152 @@ val th = Q.store_thm("assign_FP_cmp",
   \\ TRY (match_mp_tac memory_rel_Boolv_T)
   \\ TRY (match_mp_tac memory_rel_Boolv_F)
   \\ fs []);
+
+val th = Q.store_thm("assign_FP_top",
+  `(?fpt. op = FP_top fpt) ==> ^assign_thm_goal`,
+  rpt strip_tac \\ drule0 (evaluate_GiveUp |> GEN_ALL) \\ rw [] \\ fs []
+  \\ `t.termdep <> 0` by fs[]
+  \\ imp_res_tac state_rel_cut_IMP \\ pop_assum mp_tac
+  \\ qpat_x_assum `state_rel c l1 l2 s t [] locs` kall_tac \\ strip_tac
+  \\ imp_res_tac get_vars_IMP_LENGTH
+  \\ fs[do_app]
+  \\ every_case_tac \\ fs[]
+  \\ clean_tac
+  \\ imp_res_tac state_rel_get_vars_IMP
+  \\ fs[quantHeuristicsTheory.LIST_LENGTH_3]
+  \\ clean_tac
+  \\ fs[state_rel_thm] \\ eval_tac
+  \\ full_simp_tac std_ss [GSYM APPEND_ASSOC]
+  \\ rpt_drule0 (memory_rel_get_vars_IMP |> GEN_ALL)
+  \\ strip_tac
+  \\ fs[wordSemTheory.get_vars_def]
+  \\ every_case_tac \\ fs[] \\ clean_tac
+  \\ drule0 memory_rel_Word64_IMP
+  \\ imp_res_tac memory_rel_tl
+  \\ drule0 memory_rel_Word64_IMP
+  \\ imp_res_tac memory_rel_tl
+  \\ drule0 memory_rel_Word64_IMP
+  \\ qhdtm_x_assum`memory_rel`kall_tac
+  \\ simp[] \\ ntac 3 strip_tac
+  \\ clean_tac
+  \\ simp [assign_FP_top]
+  \\ TOP_CASE_TAC THEN1 fs []
+  \\ Cases_on `dimindex (:'a) = 64` \\ simp [] THEN1
+   (TOP_CASE_TAC \\ fs [] \\ clean_tac
+    \\ `shift_length c < dimindex (:α)` by (fs [memory_rel_def] \\ NO_TAC)
+    \\ rpt_drule0 get_var_get_real_addr_lemma
+    \\ once_rewrite_tac [list_Seq_def] \\ eval_tac
+    \\ qmatch_goalsub_abbrev_tac `evaluate (_,t1)`
+
+    \\ `get_var (adjust_var e2) t1 =
+         SOME (Word (get_addr c ptr' (Word 0w)))` by
+         (unabbrev_all_tac \\ fs [wordSemTheory.get_var_def,lookup_insert])
+    \\ rpt_drule0 get_var_get_real_addr_lemma
+    \\ once_rewrite_tac [list_Seq_def] \\ eval_tac
+    \\ simp [Abbr `t1`]
+
+    \\ qmatch_goalsub_abbrev_tac `evaluate (_,t2)`
+    \\ `get_var (adjust_var e3) t2 =
+         SOME (Word (get_addr c ptr (Word 0w)))` by
+         (unabbrev_all_tac \\ fs [wordSemTheory.get_var_def,lookup_insert])
+    \\ rpt_drule0 get_var_get_real_addr_lemma
+    \\ once_rewrite_tac [list_Seq_def] \\ eval_tac
+    \\ simp [Abbr `t2`]
+    \\ rpt (disch_then kall_tac)
+
+    \\ Cases_on `fpt`
+    >- (fs [fp_top_inst_def]
+    \\ rewrite_tac [list_Seq_def] \\ eval_tac
+    \\ fs [wordSemTheory.inst_def,wordSemTheory.get_var_def,lookup_insert,
+           wordSemTheory.set_fp_var_def,wordSemTheory.get_fp_var_def,
+           FLOOKUP_UPDATE,wordSemTheory.set_var_def,w2w_select_id,
+           fpSemTheory.fp_top_def]
+    \\ assume_tac(GEN_ALL evaluate_WriteWord64)
+    \\ SEP_I_TAC "evaluate" \\ fs[]
+    \\ full_simp_tac std_ss [GSYM APPEND_ASSOC,GSYM join_env_locals_def]
+    \\ first_x_assum drule0
+    \\ simp[wordSemTheory.get_var_def]
+    \\ fs[lookup_insert,good_dimindex_def,consume_space_def]
+    \\ strip_tac
+    \\ clean_tac \\ fs[]
+    \\ `1 < x.space` by (cheat) (* FIXME *)
+    \\ fs[]
+    \\ conj_tac \\ TRY (rw [] \\ NO_TAC)
+    \\ fs [FAPPLY_FUPDATE_THM] \\ rfs [w2w_w2w_64]
+    \\ rpt_drule0 memory_rel_less_space
+    \\ disch_then match_mp_tac \\ fs [])
+
+    \\ `get_var (adjust_var e2) t1 =
+         SOME (Word (get_addr c ptr' (Word 0w)))` by
+         (unabbrev_all_tac \\ fs [wordSemTheory.get_var_def,lookup_insert])
+    \\ once_rewrite_tac [list_Seq_def] \\ eval_tac
+    \\ `get_var (adjust_var e3) t1 =
+         SOME (Word (get_addr c ptr (Word 0w)))` by
+         (unabbrev_all_tac \\ fs [wordSemTheory.get_var_def,lookup_insert])
+    \\ rpt_drule0 get_var_get_real_addr_lemma
+    \\ once_rewrite_tac [list_Seq_def] \\ eval_tac
+    \\ simp [Abbr `t1`]
+    \\ rpt (disch_then kall_tac)
+    \\ once_rewrite_tac [list_Seq_def] \\ eval_tac
+    \\ once_rewrite_tac [list_Seq_def] \\ eval_tac
+    \\ Cases_on `fpt` \\ fs [fp_top_inst_def]
+    \\ rewrite_tac [list_Seq_def] \\ eval_tac
+    \\ fs [wordSemTheory.inst_def,wordSemTheory.get_var_def,lookup_insert,
+           wordSemTheory.set_fp_var_def,wordSemTheory.get_fp_var_def,
+           FLOOKUP_UPDATE,wordSemTheory.set_var_def,w2w_select_id,
+           fpSemTheory.fp_top_def]
+    \\ assume_tac(GEN_ALL evaluate_WriteWord64)
+    \\ SEP_I_TAC "evaluate" \\ fs[]
+    \\ full_simp_tac std_ss [GSYM APPEND_ASSOC,GSYM join_env_locals_def]
+    \\ first_x_assum drule0
+    \\ simp[wordSemTheory.get_var_def]
+    \\ fs[lookup_insert,good_dimindex_def,consume_space_def]
+    \\ strip_tac
+    \\ clean_tac \\ fs[]
+    \\ conj_tac \\ TRY (rw [] \\ NO_TAC)
+    \\ fs [FAPPLY_FUPDATE_THM] \\ rfs [w2w_w2w_64]
+    \\ rpt_drule0 memory_rel_less_space
+    \\ disch_then match_mp_tac \\ fs [])
+  \\ TOP_CASE_TAC \\ fs []
+  \\ `dimindex (:'a) = 32` by rfs [good_dimindex_def] \\ fs [] \\ rveq
+  \\ eval_tac
+  \\ `shift_length c < dimindex (:α)` by (fs [memory_rel_def] \\ NO_TAC)
+  \\ once_rewrite_tac [list_Seq_def] \\ eval_tac
+  \\ qpat_x_assum `get_var (adjust_var e1) t =
+       SOME (Word (get_addr c _ (Word 0w)))` assume_tac
+  \\ rpt_drule0 get_var_get_real_addr_lemma
+  \\ qpat_x_assum `get_var (adjust_var e2) t =
+       SOME (Word (get_addr c _ (Word 0w)))` assume_tac
+  \\ rpt_drule0 get_var_get_real_addr_lemma
+  \\ qpat_abbrev_tac `t1 = t with locals := insert 15 _ t.locals`
+  \\ `get_var (adjust_var e2) t1 =
+       SOME (Word (get_addr c ptr (Word 0w)))` by
+   (fs [wordSemTheory.get_var_def,Abbr`t1`,lookup_insert]
+    \\ rw [] \\ `EVEN 15` by metis_tac [EVEN_adjust_var] \\ fs [])
+  \\ rpt_drule0 get_var_get_real_addr_lemma
+  \\ fs [Abbr`t1`]
+  \\ Cases_on `fpb` \\ fs [fp_bop_inst_def]
+  \\ rewrite_tac [list_Seq_def] \\ eval_tac
+  \\ fs [wordSemTheory.inst_def,wordSemTheory.get_var_def,lookup_insert,
+         wordSemTheory.set_fp_var_def,wordSemTheory.get_fp_var_def,
+         FLOOKUP_UPDATE,wordSemTheory.set_var_def,w2w_select_id,
+         fpSemTheory.fp_bop_def,WORD_MUL_LSL]
+  \\ rpt (disch_then kall_tac)
+  \\ assume_tac(GEN_ALL evaluate_WriteWord64_on_32)
+  \\ SEP_I_TAC "evaluate" \\ fs[]
+  \\ full_simp_tac std_ss [GSYM APPEND_ASSOC,GSYM join_env_locals_def]
+  \\ first_x_assum drule0
+  \\ simp[wordSemTheory.get_var_def]
+  \\ fs[lookup_insert,good_dimindex_def,consume_space_def]
+  \\ rfs [extract_append_id]
+  \\ (qpat_abbrev_tac `ww = fp64_add _ _ _`
+      ORELSE qpat_abbrev_tac `ww = fp64_sub _ _ _`
+      ORELSE qpat_abbrev_tac `ww = fp64_mul _ _ _`
+      ORELSE qpat_abbrev_tac `ww = fp64_div _ _ _`)
+  \\ disch_then (qspec_then `ww` mp_tac) \\ fs []
+  \\ TRY impl_tac \\ TRY (rw [] \\ NO_TAC)
+  \\ strip_tac \\ fs [FAPPLY_FUPDATE_THM]
+  \\ rveq \\ fs [] \\ rw []);
 
 val th = Q.store_thm("assign_FP_bop",
   `(?fpb. op = FP_bop fpb) ==> ^assign_thm_goal`,
